examples/pseudo_bool/pb_checkScript.sml
@@ -1,0 +1,142 @@
+(*
+  Pseudo-boolean constraints proof format and checker
+*)
+open preamble pb_constraintTheory;
+
+val _ = new_theory "pb_check";
+
+val _ = numLib.prefer_num();
+
+(* pbp = pseudo-boolean proof format
+  Below, nums represent ConstraintIds, which are 1-indexed (although 0s internally work fine)
+*)
+Datatype:
+  constr =
+  | Id num              (* Constraints can refer to earlier IDs *)
+  | Add constr constr   (* Add two constraints *)
+  | Mul constr num      (* Multiply by a constant factor *)
+  | Div constr num      (* Divide by a constant factor *)
+  | Sat constr          (* Saturation *)
+  | Lit lit             (* Literal axiom lit ≥ 0 *)
+  | Weak constr var     (* Addition of literal axioms until "var" disappears *)
+End
+
+Datatype:
+  pbpstep =
+  | Contradiction num (* Id representing a contradiction *)
+  | Delete (num list) (* Ids to to delete *)
+  | Polish constr     (* Adds a constraint, written in reverse polish notation *)
+  (* TODO below
+  | RUP constr
+  | ... *)
+End
+
+(*
+  The type of PB formulas represented as a finite map
+  num -> pb_constraint
+*)
+Type pbf = ``:pb_constraint spt``;
+Type pbp = ``:pbpstep list``;
+
+(* Computes the LHS term of the slack of a constraint under
+  a partial assignment p (list of literals) *)
+Definition lslack_def:
+  lslack (PBC ls num) p =
+  SUM (MAP FST (FILTER (λ(a,b). ¬MEM (negate b) p) ls))
+End
+
+Definition check_contradiction_def:
+  check_contradiction (PBC ls num) =
+  let l = lslack (PBC ls num) [] in
+    l < num
+End
+
+Definition check_polish_def:
+  (check_polish fml (Id n) = lookup n fml) ∧
+  (check_polish fml (Add c1 c2) =
+    OPTION_MAP2 add (check_polish fml c1) (check_polish fml c2)) ∧
+  (check_polish fml (Mul c k) =
+       OPTION_MAP (λc. multiply c k) (check_polish fml c)) ∧
+  (check_polish fml (Div c k) =
+    if k ≠ 0 then
+      OPTION_MAP (λc. divide c k) (check_polish fml c)
+    else NONE) ∧
+  (check_polish fml (Sat c) =
+    OPTION_MAP saturate (check_polish fml c)) ∧
+  (check_polish fml (Lit l) = SOME (PBC [(1,l)] 0)) ∧
+  (check_polish fml (Weak c var) =
+    OPTION_MAP (λc. weaken c var) (check_polish fml c))
+End
+
+(* The result is either:
+  Unsat -> unsatisfiability proved
+  Fail -> proof step failed (more errors can be added in imperative part)
+  Cont (pbf,num) -> continue with pbf and next ID (input formula is sat equiv to the pbv)
+*)
+Datatype:
+  pbpres = Unsat | Fail | Cont pbf num
+End
+
+Definition check_pbpstep_def:
+  check_pbpstep (step:pbpstep) (fml:pbf) (id:num) =
+  case step of
+    Contradiction n =>
+      (case lookup n fml of
+        NONE => Fail
+      | SOME c =>
+      if check_contradiction c then Unsat else Fail)
+  | Delete ls =>
+      Cont (FOLDL (λa b. delete b a) fml ls) id
+  | Polish constr =>
+    case check_polish fml constr of
+      NONE => Fail
+    | SOME c => Cont (insert id c fml) (id+1)
+End
+
+(* Copied from satSem: this is the set of pseudoboolean constraints *)
+(* TODO: probably move *)
+Definition values_def:
+  values s = {v | ∃n. lookup n s = SOME v}
+End
+
+(* TODO: every constraint is satisfied, maybe rename eval_pbc to satisfies_pbc *)
+Definition satisfies_def:
+  satisfies w pbf ⇔
+  ∀c. c ∈ values pbf ⇒ eval_pbc w c
+End
+
+Theorem check_polish_correct:
+  ∀n c w.
+  check_polish fml n = SOME c ∧ satisfies w fml ⇒
+  eval_pbc w c
+Proof
+  Induct_on`n`>>rw[check_polish_def]
+  >- (
+    (*Id case*)
+    fs[satisfies_def,values_def]>>metis_tac[])
+  >- (
+    (* add case *)
+    match_mp_tac add_thm>>
+    metis_tac[])
+ >- (
+    (* multiply case *)
+    match_mp_tac multiply_thm>>
+    metis_tac[])
+  >- (
+    (* divide case *)
+    match_mp_tac divide_thm>>
+    metis_tac[])
+  >- (
+    (* saturate case *)
+    match_mp_tac saturate_thm>>
+    metis_tac[])
+  >- (
+    (* literal case *)
+    EVAL_TAC)
+  >- (
+    (* weaken case *)
+    match_mp_tac weaken_thm>>
+    metis_tac[])
+QED
+
+val _ = export_theory ();
