examples/pseudo_bool/README.md
@@ -1,4 +1,7 @@
 A checker for pseudo-boolean constraints
 
+[pb_checkScript.sml](pb_checkScript.sml):
+Pseudo-boolean constraints proof format and checker
+
 [pb_constraintScript.sml](pb_constraintScript.sml):
 A formalisation of pseudo-boolean constraints
